\documentclass{article}
\usepackage{amssymb, amsmath}
\usepackage[hidelinks]{hyperref}
\usepackage[margin=1in]{geometry}

\setcounter{secnumdepth}{0}

\title{Chapter 4 -- Higher-Order Differential Equations}
\author{Eric Johansson}

\newcommand*\dif{\mathop{}\!\mathrm{d}}
\begin{document}
\maketitle
\tableofcontents
\newpage

\section{Chapter 4.1 -- Preliminary Theory for Linear Equations }


\subsection{4.1.7}
\begin{align*}
    x(t) &= x_0\cos (\omega t)+\frac{x_1}{\omega}\sin (\omega t)\\
    x'(t) &= -x_0 \omega\sin(\omega t)+x_1\cos  (\omega t)\\\\
    x(0)  = x_0 \Rightarrow   x_0   &= x_0\cos (0)+\frac{x_1}{\omega}\sin (0) = x_0\cdot 1+\frac{x_1}{\omega}\cdot 0 = x_0\\
    x'(0)  = x_1 \Rightarrow x_1 &= x_1\cos (0)-x_0\omega\sin (0) = x_1 \cdot 1 - x_0\omega\cdot 0   = x_1
\end{align*}

\subsection{4.1.10}
\begin{align*}
    y''+(\tan x)y &= e^{x}\\
    \frac{y''}{\tan x}+y &= \frac{e^{x}}{\tan x} \\
    \text{For the equation to have a solution the}& \text{ coefficient of \(y''\) needs to not be 0 on the interval}\\
    \text{The interval around 0 where } &\frac{1}{\tan x}\neq 0\text{ is } \left(-\frac{\pi}{2},\frac{\pi}{2}\right)
\end{align*}

\subsection{4.1.13}
\begin{align*}
    y &= c_1e^{x}\cos x+c_2e^{x}\sin x\\
    y' &= c_1e^{x}\cos x-c_1e^{x}\sin x+c_2e^{x}\sin x+c_2e^{x}\cos x\\
\end{align*}
(a)
\begin{align*}
    y(0) &= 1 \Rightarrow c_1e^{0}\cos 0+c_2e^{0}\sin 0  = 1 \Rightarrow c_1  = 1\\
    y'(\pi) &= 0 \Rightarrow e^{\pi}\cos (\pi)-e^{\pi}\sin \pi + c_2e^{\pi}\sin (\pi)+c_2e^{\pi}\cos \pi  = -e^{\pi}-c_2e^{\pi} = 0 \Rightarrow c_2 = -1\\\\
    y &= e^{x}\cos x-e^{x}\sin x
\end{align*}
(b)
\begin{align*}
    y(0) &= 1 \Rightarrow c_1e^{0}\cos 0+c_2e^{0}\sin 0  = 1 \Rightarrow c_1  = 1\\
    y(\pi)  &= -1 \Rightarrow e^{\pi}\cos \pi +c_2e^{\pi}\sin \pi  = -e^{\pi} \neq -1\\\\
    \text{No solution}
\end{align*}
(c)
\begin{align*}
    y(0) &= 1 \Rightarrow c_1e^{0}\cos 0+c_2e^{0}\sin 0  = 1 \Rightarrow c_1  = 1\\
    y\left(\frac{\pi}{2}\right)  &= 1 \Rightarrow e^{\frac{\pi}{2}}\cos \frac{\pi}{2} +c_2e^{\frac{\pi}{2}}\sin \frac{\pi}{2} = c_2e^{\frac{\pi}{2}} = 1 \Rightarrow c_2 = e^{-\frac{\pi}{2}}\\\\
    y &= e^{x}\cos x-e^{-\frac{\pi}{2}}e^{x}\sin x
\end{align*}
(d)
\begin{align*}
    y(0) &= 0 \Rightarrow c_1e^{0}\cos 0+c_2e^{0}\sin 0  = 0 \Rightarrow c_1  = 0\\
    y(\pi)  &= 0 \Rightarrow  +c_2e^{\pi}\sin \pi  = 0 \Rightarrow c_2 \in \mathbb{R} \\\\
    y &= c_2e^{x}\sin x
\end{align*}

\subsection{4.1.17}
\begin{align*}
    \frac{1}{5}f_1(x)-f_2(x) &= 1-\cos ^2x = \sin ^2x = f_3(x)
\end{align*}

\subsection{4.1.18}
\begin{align*}
    2f_3(x)-f_2(x) &= 2\cos ^2x-1 = 2\cos ^2x-\cos ^2x-\sin ^2x = \cos ^2x-\sin ^2x = \cos 2x
\end{align*}

\subsection{4.1.19}
\begin{align*}
    4f_1(x)-3f_2(x) &= 4x-3(x-1)  = 4x-3x+3 = x+3 = f_3(x)
\end{align*}

\subsection{4.1.20}
Independent

\subsection{4.1.21}
Independent, can't create \( x^2 \)

\subsection{4.1.23}
Both functions satisfy the differential equation.
\[
    W(e^{-3x},e^{4x})= \begin{pmatrix} e^{-3x}&e^{4x}\\-3e^{-3x} & 4e^{4x}\end{pmatrix}=7e^{x}\neq0 
\]

\subsection{4.1.25}
Both functions satisfy the differential equation.
\[
    W(e^{x}\cos 2x,e^{x}\sin 2x)=\begin{pmatrix}e^{x}\cos 2x & e^{x}\sin 2x \\ e^{x}\cos 2x-2e^{x}\sin 2x & e^{x}\sin 2x+2e^{x}\cos 2x \end{pmatrix} \quad x=0 \Rightarrow \begin{pmatrix}1 & 0 \\ 1 & 2\end{pmatrix} =2 \neq 0
\]

\subsection{4.1.26}
Both functions satisfy the differential equation.
\[
    W(e^{\frac{x}{2}},xe^{\frac{x}{2}})=\begin{pmatrix} e^{\frac{x}{2}} & xe^{\frac{x}{2}}\\ \frac{e^{\frac{x}{2}}}{2} & e^{\frac{x}{2}}+\frac{xe^{\frac{x}{2}}}{2} \end{pmatrix} \quad x=0 \Rightarrow \begin{pmatrix} 1 & 0 \\ 0 & 1 \end{pmatrix} = 2 \neq 0
\]

\subsection{4.1.29}
All of the functions satisfy the differential equation.
\[
    W(x,x^{-2},x^{-2}\ln x)=\begin{pmatrix}x&x^{-2}&x^{-2}\ln x\\1&-2x^{-3}&\frac{-2 \ln (x) +1}{x^3}\\0 & 6x^{-4} & -\frac{-6 \ln (x)+5}{x^4}\end{pmatrix} \quad x=1 \Rightarrow \begin{pmatrix}1&1&0\\1&-2&1\\0 & 6 & -5\end{pmatrix}=9 \neq 0
\]

\subsection{4.1.35}
(a)
\begin{align*}
    LHS=12e^{2x}-6\cdot6e^{2x}+5\cdot3e^{2x}  &= e^{2x}(12-36+15)=-9e^{2x}=RHS\\\\
    LHS=2-6(2x+3)+5(x^2+3x) &= 5x^2+15x-12x+2-18=5x^2+3x-16=RHS 
\end{align*}
(b)
\begin{align*}
    y_{p_1}+y_{p_2} &= 5x^2+3x-16-3e^{2x}\\\\
    -\frac{y_{p_1}}{9}-2y_{p_2} &= -2x^2-6x-\frac{e^{2x}}{3}
\end{align*}

    
\section{Chapter 4.2 -- Reduction of Order}

\subsection{4.2.9}
\begin{align*}
    x^2y''+2xy'-6y &= 0; \quad y_1 = x^4\\
    y''-\frac{7y'}{x}+\frac{16y}{x^2}  &= 0; \quad P = -\frac{7}{x}  \\
    y_2 &= y_1(x) \int \frac{e^{-\int P(x) \; \mathrm{d}x}}{y_1^2(x)} \; \mathrm{d}x\\
    y_2 &= x^4 \int \frac{e^{-\int -\frac{7}{x} \; \mathrm{d}x}}{x^8} \; \mathrm{d}x\\
    y_2 &= x^4 \int \frac{e^{7\int \frac{1}{x} \; \mathrm{d}x}}{x^8} \; \mathrm{d}x\\
    y_2 &= x^4 \int \frac{e^{7 \ln\left|x\right|}}{x^8} \; \mathrm{d}x\\
    y_2 &= x^4 \int \frac{e^{7 \ln\left|x\right|}}{x^8} \; \mathrm{d}x\\
    y_2 &= x^4 \int \frac{e^{ \ln\left|x^7\right|}}{x^8} \; \mathrm{d}x\\
    y_2 &= x^4 \int \frac{x^7}{x^8} \; \mathrm{d}x\\
    y_2 &= x^4 \int \frac{1}{x} \; \mathrm{d}x\\
    y_2 &= x^4 \ln\left|x\right|
\end{align*}

\subsection{4.2.10}
\begin{align*}
    x^2y''+2xy'-6y &= 0; \quad y_1 = x^2\\ 
    y''+\frac{2y'}{x}-\frac{6y}{x^2} &= 0; \quad P = \frac{2}{x}\\
    y_2 &=x^2\int \frac{e^{-\int \frac{2}{x} \; \mathrm{d}x}}{x^4} \; \mathrm{d}x\\
    y_2 &=x^2\int \frac{e^{\ln\left|x^{-2}\right|}}{x^4} \; \mathrm{d}x\\
    y_2 &=x^2\int \frac{1}{x^6} \; \mathrm{d}x\\
    y_2 &= x^2 \cdot \frac{-1}{5x^5}\\
    y_2 &= -\frac{1}{5x^3}
\end{align*}
        
\newpage
\subsection{4.2.19}
\begin{align*}
    y''-3y'+2y &= 5e^{3x}; \quad y_1 = e^{x}\\
    y_2 &= e^{x}\int \frac{e^{-\int -3 \; \mathrm{d}x}}{e^{2x}} \; \mathrm{d}x\\
    y_2 &= e^{x}\int e^{x}\; \mathrm{d}x\\
    y_2 &= e^{2x}\\
    y_p &= Ae^{3x}\\
    9Ae^{3x}-9Ae^{3x}+2Ae^{3x} &= 5e^{3x}\\
    2A &= 5\\
    A &= \frac{5}{2}\\
    y_p &= \frac{5e^{3x}}{2}        
\end{align*}

\subsection{4.2.20}
\begin{align*}
    y''-4y'+3y &= x; \quad y_1 = e^{x}\\
    y_2 &= e^{x}\int \frac{e^{-\int -4 \; \mathrm{d}x}}{e^{2x}} \; \mathrm{d}x\\
    y_2  &= e^{3x}\\
    y_p  &= ax^2+bx+c\\
    2a-4(2ax+b)+3(ax^2+bx+c) &= x\\
    &\begin{pmatrix}2a&-4b&3c|&0\\ 8a & 3b & 0 | & 1 \\ 3a & 0 & 0 |& 0 \end{pmatrix}\\
    a=0 \quad b &= \frac{1}{3} \quad c = \frac{4}{9}\\
    y_p  &= \frac{x}{3}+\frac{4}{9}
\end{align*}


\section{Chapter 4.6 -- Variation of Parameters}

\subsection{4.6.1}
\begin{align*}
    y''+y &= \sec x\\
    m^2+1 &= 0 \Rightarrow m = \pm i\\
    y_c &= c_1\cos x+c_2\sin x\\\\
    W(\cos x,\sin x)  &= \begin{vmatrix}\cos x & \sin x \\ -\sin x & \cos x \end{vmatrix} = \cos ^2+\sin ^2 = 1\\
    W_1 &= \begin{vmatrix} 0 & \sin x \\ \sec x & \cos x\end{vmatrix} = -\sin x \sec x = -\tan x\\
    W_2 &= \begin{vmatrix} \cos x & 0\\ -\sin x & \sec x\end{vmatrix} = \cos x \sec x = 1\\
    u_1' &= \frac{W_1}{W}= \frac{-\tan x}{1} \Rightarrow u_1 =  \ln\left|\cos x\right|\\
    u_2' &= \frac{W_2}{W}= \frac{1}{1} \Rightarrow u_2 = x\\
    y_p &= \cos x\ln\left|\cos x\right|+x\sin x\\\\
    y  = y_c+y_p&= c_1\cos x+c_2\sin x+\cos x \ln\left|\cos x\right|+x\sin x
\end{align*}



\subsection{4.6.6}
\begin{align*}
    y''+y &= \sec^2x\\
    y_c &= c_1\cos x+c_2\sin x\\\\
    W(\cos x,\sin x)  &= \begin{vmatrix}\cos x & \sin x \\ -\sin x & \cos x \end{vmatrix} = \cos ^2+\sin ^2 = 1\\
    W_1 &= \begin{vmatrix} 0 & \sin x \\ \sec^2 x & \cos x\end{vmatrix} = -\sin x \sec^2x  =- \tan x \sec x\\
    W_2 &= \begin{vmatrix} \cos x & 0\\ -\sin x & \sec^2 x\end{vmatrix} = \cos x\sec^2x = \sec x\\
    u_1' &= \frac{W_1}{W} = \frac{-\tan x \sec x}{1} =  -\tan x\sec  x \Rightarrow u_1 =-\sec x\\
    u_2' &= \frac{W_2}{W} = \frac{\sec x }{1}  = \sec x \Rightarrow u_2  = \ln\left|\sec x + \tan x\right|\\
    y_p &= -\sec x \cos x + \ln\left|\sec x + \tan x\right| = -1+\ln\left|\sec x + \tan x\right|\\\\
    y &= y_c+y_p =  c_1\cos x+c_2\sin x  -1+\ln\left|\sec x + \tan x\right|\sin x
\end{align*}

\subsection{4.6.11}
\begin{align*}
    y''+3y'+2y &= \frac{1}{1+e^{x}}\\
    y_c &= c_1e^{-x}+c_2e^{-2x}\\\\
    W(e^{x},e^{2x}) &=  \begin{vmatrix}e^{-x} & e^{-2x}\\ e^{-x}& -2e^{-2x}\end{vmatrix} = -2e^{-3x}+e^{-3x}  = -e^{-3x}\\
    W_1 &= \begin{vmatrix} 0 & e^{-2x}\\ \frac{1}{1+e^{x}}  &-2e^{-2x}\end{vmatrix} = \frac{e^{-2x}}{1+e^{x}}     \\
    W_2 &= \begin{vmatrix} e^{-x} & 0\\ e^{-x} & \frac{1}{1+e^{x}} \end{vmatrix} = \frac{e^{-x}}{1+e^{x}}\\  
    u_1' &= \frac{W_1}{W}  = \frac{\frac{e^{-2x}}{1+e^{x}}}{e^{-3x}} =  \frac{e^{x}}{1+e^{x}}  \Rightarrow u_1  = \ln\left(1+e^{x}\right)     \\
    u_2' &= \frac{W_1}{W}  = \frac{\frac{e^{-x}}{1+e^{x}}}{e^{-3x}} = \frac{e^{2x}}{1+e^{x}}\Rightarrow u_2 = \ln\left(1+e^{x}\right)-1-e^{x}\\
    y_p  &= e^{-x}\ln\left(1+e^{x}\right)-e^{-x}-e^{-2x}+e^{-2x}\ln\left(1+e^{x}\right) \\
(\text{Ignore \( e^{-x} \) and \( e^{-2x} \)}&\text{ when adding to solution because they are already present in \( y_c \) }) \\\\
    y &= y_c+y_p = c_1e^{-x}+c_2e^{-2x}+ e^{-x}\ln\left(1+e^{x}\right)+e^{-2x}\ln\left(1+e^{x}\right)
\end{align*}

\subsection{4.6.27}
\begin{align*}
    x^2y''+xy'+\left(x^2-\frac{1}{4}\right)y &= x^{\frac{3}{2}}\\
    y_1 = x^{-\frac{1}{2}}\cos x, & \quad y_2 = x^{-\frac{1}{2}}\sin x\\
    W(x^{-\frac{1}{2}}\cos x, x^{-\frac{1}{2}}\sin x)  &= \begin{vmatrix} x^{-\frac{1}{2}}\cos x& x^{-\frac{1}{2}}\sin x \\-\frac{1}{2}x^{-\frac{3}{2}}\cos x-x^{-\frac{1}{2}}\sin x &-\frac{1}{2}x^{-\frac{3}{2}}\sin  x+x^{-\frac{1}{2}}\cos  x   \end{vmatrix} = \frac{1}{x}\\
    W_1 &= \begin{vmatrix}0 & x^{-\frac{1}{2}}\sin x \\ x^{-\frac{1}{2}} & -\frac{1}{2}x^{-\frac{3}{2}}\sin  x+x^{-\frac{1}{2}}\cos  x  \end{vmatrix}  = -\frac{\sin x}{x}\\
    W_2 &= \begin{vmatrix} x^{-\frac{1}{2}}\cos x& 0 \\-\frac{1}{2}x^{-\frac{3}{2}}\cos x-x^{-\frac{1}{2}}\sin x  & x^{-\frac{1}{2}}\end{vmatrix} = \frac{\cos x}{x}\\
    u_1' &= \frac{W_1}{W} = -\sin x \Rightarrow u_1=\cos x\\
    u_2' &= \frac{W_2}{W} = \cos x  \Rightarrow u_2=\sin x\\
    y_p &= x^{-\frac{1}{2}}\cos ^2x+x^{-\frac{1}{2}}\sin ^2x=\frac{1}{\sqrt{x}}(\cos ^2x+\sin ^2x)= \frac{1}{\sqrt{x}}\\
    y &= y_c+y_p=c_1x^{-\frac{1}{2}}\cos x+c_2x^{-\frac{1}{2}}\sin x+\frac{1}{\sqrt{x}}
\end{align*}


\subsection{4.6.28}
\begin{align*}
    x^2y''+xy'+y &= \sec (\ln x)\\
    y''+\frac{y'}{x}+\frac{y}{x^2} &= \frac{\sec (\ln x)}{x^2}\\
    W(\cos (\ln x), \sin (\ln x))  &= \begin{vmatrix}\cos (\ln x) &\sin (\ln x) \\ \frac{-\sin (\ln x)}{x} & \frac{\cos (\ln x)}{x} \end{vmatrix}=\frac{\cos ^2(\ln x)}{x}+\frac{\sin^2(\ln x)}{x}=\frac{1}{x}\\
    W_1 &= \begin{vmatrix} 0 & \sin (\ln x) \\ \frac{\sec (\ln x)}{x^2}&\frac{\cos  (\ln x)}{x} \end{vmatrix} = -\frac{\tan (\ln x)}{x^2}\\
    W_2 &= \begin{vmatrix}\cos (\ln x) & 0 \\ \frac{-\sin (\ln x)}{x}  &\frac{\sec (\ln x)}{x^2} \end{vmatrix} = \frac{1}{x^2}\\
    u_1'  &= -\frac{\tan (\ln x)}{x}  \Rightarrow u_2 = \ln\left|\cos (\ln x)\right|\\
    u_2' &= \frac{1}{x}  \Rightarrow u_1=\ln\left|x\right|\\
    y_p &= \cos (\ln x)\ln\left|\cos (\ln x)\right|+\sin (\ln x)\ln\left|x\right|\\\\
    y &= y_c+y_p=c_1\cos (\ln x)+c_2\sin (\ln x)+ \cos (\ln x)\ln\left|\cos (\ln x)\right|+\sin (\ln x)\ln\left|x\right|
\end{align*}


\end{document}

